Structures/SystemSetup.v
@@ -1,0 +1,33 @@
+From mathcomp.ssreflect
+Require Import ssreflect ssrbool ssrnat eqtype ssrfun seq fintype path.
+Require Import Eqdep.
+From fcsl
+Require Import pred prelude ordtype pcm finmap unionmap heap.
+From Toychain
+Require Import SeqFacts Chains Blocks.
+Set Implicit Arguments.
+Unset Strict Implicit.
+Unset Printing Implicit Defensive.
+Require Extraction.
+
+Parameter Hash : ordType.
+Parameter VProof : eqType.
+Parameter Transaction : eqType.
+
+Definition block: Type := @Block Hash Transaction VProof.
+Definition TxPool := seq Transaction.
+Definition Blockchain := seq block.
+Definition BlockTree := union_map Hash block.
+
+Parameter Timestamp : Type.
+Parameter Address : finType.
+Parameter GenesisBlock : block.
+Parameter hashT : Transaction -> Hash.
+Parameter hashB : block -> Hash.
+Parameter genProof : Address -> Blockchain -> TxPool -> Timestamp -> option (TxPool * VProof).
+Parameter VAF : VProof -> Blockchain -> TxPool -> bool.
+Parameter FCR : Blockchain -> Blockchain -> bool.
+
+(* Transaction is valid and consistent with the given chain *)
+Parameter txValid : Transaction -> Blockchain -> bool.
+Parameter tpExtend : TxPool -> BlockTree -> Transaction -> TxPool.
